execution/tests/EIP20Tests/EIP20TokenTests.v
@@ -10,51 +10,63 @@ From ConCert Require Import Serializable.
 From ConCert Require Import BoundedN.
 From ConCert Require Import Containers.
 From ConCert Require Import EIP20Token.
+From ConCert Require Import ResultMonad.
+From ConCert Require Import ChainedList.
 Require Import Extras.
 
 From ConCert.Execution.QCTests Require Import
   TestUtils ChainPrinters SerializablePrinters EIP20TokenPrinters EIP20TokenGens TraceGens.
 
-(* For monad notations *)
-From ExtLib.Structures Require Import Monads.
-Import MonadNotation. Open Scope monad_scope.
 From Coq Require Import List Int.
 Import BoundedN.Stdpp.
 Import LocalBlockchain.
 Import ListNotations.
-Close Scope address_scope.
 
 (* -------------------------- Tests of the EIP20 Token Implementation -------------------------- *)
 
-Definition Base := TestUtils.LocalChainBase.
-
+Existing Instance showTokenState.
 
 Definition token_setup := EIP20Token.build_setup creator (100%N).
-Definition deploy_eip20token : @ActionBody Base := create_deployment 0 EIP20Token.contract token_setup.
+Definition deploy_eip20token := create_deployment 0 EIP20Token.contract token_setup.
 
 Let contract_base_addr := BoundedN.of_Z_const AddrSize 128%Z.
 
-Definition chain_with_token_deployed :=
-  unpack_option (my_add_block lc_initial
+(* In the initial chain we transfer some assets to a few accounts, just to make the addresses
+   present in the chain state. The amount transferred is irrelevant. *)
+Definition token_cb :=
+  unpack_result (TraceGens.add_block (lcb_initial AddrSize)
   [
-    build_act creator (act_transfer person_1 10);
-    build_act creator (act_transfer person_2 10);
-    build_act creator (act_transfer person_3 10);
+    build_act creator (act_transfer person_1 0);
+    build_act creator (act_transfer person_2 0);
+    build_act creator (act_transfer person_3 0);
     build_act creator deploy_eip20token
   ]).
 
-Definition gEIP20TokenChainTraceList max_acts_per_block lc length :=
-  gLocalChainTraceList_fix lc (fun lc _ =>
-    gEIP20TokenAction lc contract_base_addr) length max_acts_per_block.
+Module TestInfo <: EIP20GensInfo.
+  Definition contract_addr := contract_base_addr.
+  Definition gAccount (c : Chain) := elems [person_1; person_2; person_3; person_4; person_5].
+End TestInfo.
+Module MG := EIP20Gens TestInfo. Import MG.
 
-Definition token_reachableFrom (lc : LocalChain) pf : Checker :=
-  @reachableFrom AddrSize lc (gEIP20TokenChainTraceList 1) pf.
+Definition gTokenChain max_acts_per_block token_cb max_length := 
+  let act_depth := 1 in 
+  gChain token_cb
+    (fun env act_depth => gEIP20TokenAction env) max_length act_depth max_acts_per_block.
+(* Sample (gTokenChain 2 token_cb 7).  *)
 
-Definition token_reachableFrom_implies_reachable (lc : LocalChain) pf1 pf2 : Checker :=
-  reachableFrom_implies_reachable lc (gEIP20TokenChainTraceList 1) pf1 pf2.
+Definition forAllTokenChainTraces n :=
+  let max_acts_per_block := 2 in
+  forAllChainState n token_cb (gTokenChain max_acts_per_block).
+
+Definition pre_post_assertion_congress P c Q :=
+  let max_acts_per_block := 2 in
+  let trace_length := 7 in
+  pre_post_assertion trace_length token_cb (gTokenChain max_acts_per_block) EIP20Token.contract c P Q.
+
+Notation "{{ P }} c {{ Q }}" := (pre_post_assertion_congress P c Q) ( at level 50).
 
 Open Scope string_scope.
-Definition debug_gEIP20Checker {A : Type}
+(* Definition debug_gEIP20Checker {A : Type}
                               `{Checkable A}
                                lc
                                (act : option Action)
@@ -63,17 +75,15 @@ Definition debug_gEIP20Checker {A : Type}
     ("lc balances: " ++ show (lc_account_balances lc) ++ sep ++ nl
     ++ show act
     ++ "token state: " ++ show (lc_token_contracts_states_deserialized lc) ++ sep ++ nl
-    ).
+    ). *)
 
 (* Sample (gEIP20TokenAction chain_with_token_deployed contract_base_addr). *)
 (* Sample (gEIP20TokenChainTraceList 1 chain_with_token_deployed 5). *)
+Close Scope string_scope.
 
 Local Open Scope N_scope.
 
-Extract Constant defNumDiscards => "(4 * defNumTests)".
-
-Definition forAllEIP20Traces n := forAllTraces n chain_with_token_deployed (gEIP20TokenChainTraceList 2).
-Notation "{{ P }} c {{ Q }}" := (pre_post_assertion 10 chain_with_token_deployed (gEIP20TokenChainTraceList 1) c P Q)( at level 50).
+Extract Constant defNumDiscards => "(3 * defNumTests)".
 
 Definition msg_is_transfer (cstate : EIP20Token.State) (msg : EIP20Token.Msg) :=
   match msg with
@@ -109,65 +119,59 @@ Definition post_transfer_correct cctx old_state msg (result_opt : option (State 
 
 (* QuickChick (
   {{msg_is_transfer}}
-  EIP20Token.contract
+  contract_base_addr
   {{post_transfer_correct}}
 ). *)
 
-(* coqtop-stdout:*** Gave up! Passed only 126 tests
-Discarded: 20000 *)
-(* coqtop-stdout:+++ Passed 10000 tests (0 discards) *)
+(* +++ Passed 10000 tests (0 discards) *)
 
 (* One key property: the sum of the balances is always equal to the initial supply *)
-Definition sum_balances_eq_init_supply lc :=
-  (* debug_gEIP20Checker lc None *)
-  let contract_states := lc_token_contracts_states_deserialized lc in
-  checker match FMap.find contract_base_addr contract_states with
-  | Some state =>
-    let balances_list := (map snd o FMap.elements) state.(balances) in
-    let balances_sum : N := fold_left N.add balances_list 0%N in
-    balances_sum =? state.(total_supply)
-  | None => false
+Definition sum_balances_eq_init_supply (state : EIP20Token.State) :=
+  let balances_list := (map snd o FMap.elements) state.(balances) in
+  let balances_sum : N := fold_left N.add balances_list 0%N in
+  balances_sum =? state.(total_supply).
+
+Definition checker_get_state {prop} `{Checkable prop} (pf : State -> prop) (cs : ChainState) : Checker := 
+  match get_contract_state EIP20Token.State cs contract_base_addr with
+  | Some state => checker (pf state)
+  | None => checker true (* trivially true case *) 
   end.
 
-(* QuickChick (forAllEIP20Traces 10 sum_balances_eq_init_supply). *)
+(* QuickChick (forAllTokenChainTraces 5 (checker_get_state sum_balances_eq_init_supply)). *)
 (* coqtop-stdout:+++ Passed 10000 tests (1570 discards) *)
 (* 8 seconds *)
 
 (* INVALID PROPERTY: accounts may allow multiple other accounts to transfer tokens, but the actual transfer ensures that
    no more tokens are sent than the balance of the sender. *)
-Definition sum_allowances_le_init_supply lc :=
-  debug_gEIP20Checker lc None
-      (match FMap.find contract_base_addr (lc_token_contracts_states_deserialized lc) with
-      | Some state =>
-        let allowances := map_values_FMap
-          (fun allowance_map => fold_left N.add ((map snd o FMap.elements) allowance_map) 0)
-          state.(allowances) in
-        let allowances_list := (map snd o FMap.elements) allowances in
-        let allowances_sum := fold_left N.add allowances_list 0%N in
-        allowances_sum <=? state.(total_supply)
-      | None => false
-      end).
+Definition sum_allowances_le_init_supply (state : EIP20Token.State) :=
+  (* debug_gEIP20Checker lc None *)
+  let allowances := map_values_FMap
+    (fun allowance_map => fold_left N.add ((map snd o FMap.elements) allowance_map) 0)
+      state.(allowances) in
+  let allowances_list := (map snd o FMap.elements) allowances in
+  let allowances_sum := fold_left N.add allowances_list 0%N in
+  allowances_sum <=? state.(total_supply).
 
 Definition sum_allowances_le_init_supply_P maxLength :=
-  forAllTraces maxLength chain_with_token_deployed (gEIP20TokenChainTraceList 2)
-    sum_allowances_le_init_supply.
+  forAllChainState maxLength token_cb (gTokenChain 2)
+    (checker_get_state sum_allowances_le_init_supply).
 
 (* QuickChick (sum_allowances_le_init_supply_P 5). *)
 
 Definition person_has_tokens person (n : N) :=
-  fun lc =>
-    match FMap.find contract_base_addr (lc_token_contracts_states_deserialized lc) with
-    | Some state => if n =? (FMap_find_ person state.(balances) 0)
-                    then Some n
-                    else None
-    | None => None
+  fun cs => 
+    match get_contract_state State cs contract_base_addr with
+    | Some state => n =? (FMap_find_ person state.(balances) 0)
+    | None => true (* trivial case *)
     end.
-
-(* Notation "lc '~~>' pf" :=
-  (token_reachableFrom lc pf)
+    
+(* Notation "cb '~~>' pf" :=
+  (reachableFrom_chaintrace cb (gTokenChain 2) pf)
   (at level 45, no associativity). *)
 
-(* QuickChick (chain_with_token_deployed ~~> person_has_tokens person_3 12). *)
+(* QuickChick (token_cb ~~> (person_has_tokens person_3 12)). *)
+
+(* QuickChick (chain_with_token_deployed ~~> (fun lc => isSome (person_has_tokens person_3 12 lc))). *)
 (* QuickChick (chain_with_token_deployed ~~> person_has_tokens creator 0). *)
 
 (* QuickChick (token_reachableFrom_implies_reachable
@@ -177,7 +181,7 @@ Definition person_has_tokens person (n : N) :=
 ). *)
 
 Notation "'{' lc '~~>' pf1 '===>' pf2 '}'" :=
-  (reachableFrom_implies_tracePropSized_new 3 lc (gEIP20TokenChainTraceList 1) pf1 pf2)
+  (reachableFrom_implies_chaintracePropSized 3 lc (gTokenChain 2) pf1 pf2)
   (at level 90, left associativity).
 
 (* This (false) property says that from the initial chain where the token contract has been deployed,
@@ -211,25 +215,20 @@ Definition get_transferFrom_act (act : Action) : option (Address * Address * EIP
   | _ => None
   end.
 
-Definition state_has_some_approve_act {AddrSize : N} (step : @LocalChainStep AddrSize) :=
-  match step with
-  | step_action prev_lc header next_lc acts =>
-    match find (isSome o get_approve_act) acts with
-    | Some x => get_approve_act x
-    | None => None
-    end
-  | _ => None
+Definition state_has_some_approve_act (cs : ChainState) :=
+  match find (isSome o get_approve_act) cs.(chain_state_queue) with
+  | Some x => get_approve_act x
+  | None => None
   end.
 
 Definition delegate_made_no_transferFroms (approve_act_p :  (Address * Address * EIP20Token.Msg))
-                                          (trace : list LocalChainStep) :=
+                                          (cs : ChainState) :=
   let caddr := fst (fst approve_act_p) in
   let approver := snd (fst approve_act_p) in
   match (snd approve_act_p) with
   | approve delegate amount =>
-    forallb (fun step =>
-      let acts := acts_of_lcstep step in
-      let act_not_transferFrom_delegate act :=
+    let acts := cs.(chain_state_queue) in
+    let act_not_transferFrom_delegate act :=
         match get_transferFrom_act act with
         | Some (caddr', caller, (transfer_from from to _)) =>
           if (address_eqb caddr' caddr)
@@ -237,15 +236,9 @@ Definition delegate_made_no_transferFroms (approve_act_p :  (Address * Address *
           else true
         | _ => true
         end in
-      forallb act_not_transferFrom_delegate acts
-    ) trace
+    forallb act_not_transferFrom_delegate acts
   | _ => false
   end.
-
-(* Definition forAnyStateInTrace n trace c :=
-  let trace' := map prev_lc_of_lcstep trace in
-  forAll (elems_ chain_with_token_deployed trace') (fun lc =>
-  forAllTraces_traceProp n lc (gEIP20TokenChainTraceList 2) c). *)
 
 Definition allower_addr (approve_act_p : (Address * Address * EIP20Token.Msg)) :=
   match snd approve_act_p with
@@ -272,8 +265,8 @@ Definition transfer_from_amount (transferFrom_act_p : (Address * Address * EIP20
   | _ => 0
   end.
 
-Definition allower_reapproves_delegate_step allower delegate step :=
-  let acts := acts_of_lcstep step in
+Definition allower_reapproves_delegate_step allower delegate (cs : ChainState) :=
+  let acts := cs.(chain_state_queue) in
   match find isSome (map get_approve_act acts) with
   | Some (Some (caddr, caller, (approve delegate' amount)) as act)  =>
     if address_eqb caller allower && address_eqb delegate delegate'
@@ -282,14 +275,14 @@ Definition allower_reapproves_delegate_step allower delegate step :=
   | _ => None
   end.
 
-Definition delegate_transferFrom_sum_of_approver approver delegate trace :=
+Definition delegate_transferFrom_sum_of_approver approver delegate (trace : list ChainState) :=
   fold_left (fun acc step =>
     let transfer_from_acts := fold_left (fun acc act =>
       match get_transferFrom_act act with
       | Some x => x :: acc
       | None => acc
       end
-    ) (acts_of_lcstep step) [] in
+    ) (step.(chain_state_queue)) [] in
     let filter_p p := if address_eqb (allower_addr p) approver
                       then match delegate_addr p with
                            | Some delegate' => address_eqb delegate delegate'
@@ -301,70 +294,63 @@ Definition delegate_transferFrom_sum_of_approver approver delegate trace :=
     step_sum + acc
   ) trace 0.
 
-Extract Constant defNumDiscards => "(3 * defNumTests)".
-
-Fixpoint last_opt {A : Type} (l : list A) : option A :=
-  match l with
-  | [] => None
-  | x::[] => Some x
-  | x::xs => last_opt xs
-  end.
-
-Definition allower_reapproves_transferFrom_correct trace allower delegate (first_approval_amount : N) :=
-  match last_opt trace with
-  | None => false ==> true
-  | Some start_step =>
-    let start_lc := next_lc_of_lcstep start_step in
-    reachableFrom_implies_tracePropSized_new 2 start_lc (gEIP20TokenChainTraceList 2)
-    (allower_reapproves_delegate_step allower delegate)
-    (fun new_approval_amount pre_trace _ =>
-      let trace_until_reapproval := app trace (removelast pre_trace) in
-      let delegate_spent_until_reapproval := delegate_transferFrom_sum_of_approver allower delegate trace_until_reapproval in
-      let delegate_spent_incl_reapproval_act :=
-        delegate_transferFrom_sum_of_approver allower delegate (trace ++ pre_trace) in
-      let total_allowed := delegate_spent_until_reapproval + new_approval_amount in
-      (new_approval_amount <? first_approval_amount) ==>
-      whenFail (show delegate ++ " spent "
-        ++ show delegate_spent_incl_reapproval_act
-        ++ " on behalf of " ++ show allower
-        ++ " when they were only allowed to spend at most "
-        ++ show total_allowed  ++ nl)
-      (delegate_spent_incl_reapproval_act <=? total_allowed)
-    )
-  end.
+Definition allower_reapproves_transferFrom_correct (pre_trace post_trace : list ChainState) allower delegate (first_approval_amount : N) :=
+  let trace := pre_trace ++ post_trace in
+  let reapprove_correct cs :=
+  (* Checks if a chainstate has a re-approval act, and if so, then checks that the spent amount inbetween
+     the first approval and the re-approval is not greater than expected. *)
+  let res := (allower_reapproves_delegate_step allower delegate cs) in
+    isSomeCheck res (fun new_approval_amount =>
+      let p := split_at_first_satisfying (isSome o (allower_reapproves_delegate_step allower delegate)) trace in
+      match p with
+      | Some (trace_until_reapproval, _) =>
+        let delegate_spent_until_reapproval := delegate_transferFrom_sum_of_approver allower delegate trace_until_reapproval in
+        let delegate_spent_incl_reapproval_act :=
+          delegate_transferFrom_sum_of_approver allower delegate trace in
+        let total_allowed := delegate_spent_until_reapproval + new_approval_amount in
+        (new_approval_amount <? first_approval_amount) ==>
+        whenFail (show delegate ++ " spent "
+          ++ show delegate_spent_incl_reapproval_act
+          ++ " on behalf of " ++ show allower
+          ++ " when they were only allowed to spend at most "
+          ++ show total_allowed  ++ nl)
+        (delegate_spent_incl_reapproval_act <=? total_allowed)
+      | None => checker false
+      end) in
+  conjoin_map reapprove_correct trace.
 
 Definition reapprove_transfer_from_safe_P :=
-  (reachableFrom_implies_tracePropSized_new 3 chain_with_token_deployed (gEIP20TokenChainTraceList 2))
-  state_has_some_approve_act
+  {token_cb ~~> state_has_some_approve_act ===>
   (fun approve_act_p pre_trace post_trace =>
-    (* (delegate_made_no_transferFroms approve_act_p post_trace   *)
     isSomeCheck (delegate_addr approve_act_p) (fun delegate =>
-      allower_reapproves_transferFrom_correct post_trace
+      allower_reapproves_transferFrom_correct pre_trace
+                                              post_trace
                                               (allower_addr approve_act_p)
                                               delegate
-                                              (approve_amount approve_act_p)
-      )
-    (* ) *)
-  ).
+                                              (approve_amount approve_act_p)))}.
 
 (* QuickChick reapprove_transfer_from_safe_P. *)
 
-(* coqtop-stdout:Begin Trace:
+(* 
+Chain{| 
+Block 1 [
+Action{act_from: 10%256, act_body: (act_transfer 11%256, 0)};
+Action{act_from: 10%256, act_body: (act_transfer 12%256, 0)};
+Action{act_from: 10%256, act_body: (act_transfer 13%256, 0)};
+Action{act_from: 10%256, act_body: (act_deploy 0, transfer 10%256 100)}];
+Block 2 [
+Action{act_from: 10%256, act_body: (act_call 128%256, 0, transfer 11%256 7)};
+Action{act_from: 10%256, act_body: (act_call 128%256, 0, transfer 12%256 34)}];
+Block 3 [
+Action{act_from: 10%256, act_body: (act_call 128%256, 0, approve 12%256 32)};
+Action{act_from: 10%256, act_body: (act_call 128%256, 0, approve 11%256 23)}];
+Block 4 [
+Action{act_from: 12%256, act_body: (act_call 128%256, 0, transfer_from 10%256 10%256 25)};
+Action{act_from: 10%256, act_body: (act_call 128%256, 0, approve 12%256 8)}];|}
 
-coqtop-stdout:step_action{Action{act_from: 10%256, act_body: (act_call 128%256, 0, transfer_from 12%256 12%256 7)};
+12%256 spent 25 on behalf of 10%256 when they were only allowed to spend at most 8
 
-coqtop-stdout:Action{act_from: 12%256, act_body: (act_call 128%256, 0, approve 10%256 6)}};;
+*** Failed after 1 tests and 0 shrinks. (216 discards)
+*)
 
-coqtop-stdout:step_action{Action{act_from: 11%256, act_body: (act_call 128%256, 0, approve 10%256 1)};
-
-coqtop-stdout:Action{act_from: 12%256, act_body: (act_call 128%256, 0, approve 11%256 7)}}
-
-coqtop-stdout:End Trace
-
-coqtop-stdout:10%256 spent 7 on behalf of 12%256 when they were only allowed to spend at most 6
-
-coqtop-stdout:
-
-coqtop-stdout:*** Failed after 15 tests and 0 shrinks. (402 discards) *)
-
-(* Definition transfer_from_reduces_balance_correctly_P := . *)
+(* Definition transfer_from_reduces_balance_correctly_P := TODO... *)
