embedding/examples/crowdfunding/CrowdfundingData.v
@@ -44,7 +44,6 @@ Definition state_syn : global_dec :=
 
 Unset Printing Notations.
 
-(* Print state_syn. *)
 (* state_syn =
     gdInd State O
       (cons
@@ -63,7 +62,6 @@ Set Nonrecursive Elimination Schemes.
 Make Inductive (global_to_tc state_syn).
 
 (** As a result, we get a new Coq record [State_coq] *)
-(* Print State_coq. *)
 
 Definition msg_syn :=
   [\ data Msg =
