execution/tests/CongressTests/CongressPrinters.v
@@ -1,26 +1,17 @@
-From ConCert Require Import Blockchain LocalBlockchain Congress.
+From ConCert Require Import Blockchain Congress.
 From ConCert Require Import Serializable.
-From ConCert Require Import BoundedN ChainedList.
-From ConCert.Execution.QCTests Require Import TestUtils ChainPrinters.
-
-Require Import ZArith Strings.String.
+From ConCert.Execution.QCTests Require Import TestUtils.
 
 From QuickChick Require Import QuickChick. Import QcNotation.
-From ExtLib.Structures Require Import Functor Applicative.
-From ExtLib.Structures Require Import Monads.
-Import MonadNotation. Open Scope monad_scope.
 From Coq Require Import List. Import ListNotations.
-From Coq Require Import Strings.BinaryString.
-From Coq Require Import Morphisms.
-From Coq Require Import Program.Basics.
-Require Import Containers.
-Notation "f 'o' g" := (compose f g) (at level 50).
-Definition LocalChainBase : ChainBase := TestUtils.LocalChainBase.
 Open Scope string_scope.
 
 Arguments SerializedValue : clear implicits.
 Arguments deserialize : clear implicits.
 Arguments serialize : clear implicits.
+
+Section CongressPrinters.
+Context `{Show Address}.
 
 Instance showRules : Show Rules :=
 {|
@@ -32,15 +23,15 @@ Instance showRules : Show Rules :=
     ++ "}"
 |}.
 
-Definition string_of_ca str_of_msg ca :=
-match ca with
-| cact_transfer to amount => "(transfer: " ++ show to ++ sep ++ show amount ++ ")"
-| cact_call to amount msg => "(call: " ++ show to ++ sep ++ show amount ++ sep ++
-    match @deserialize Msg _ msg with
-    | Some msg => str_of_msg msg
-    | None =>  "<FAILED DESERIALIZATION>"
-    end ++ ")"
-end.
+Definition string_of_ca (str_of_msg : Msg -> string) ca :=
+  match ca with
+  | cact_transfer to amount => "(transfer: " ++ show to ++ sep ++ show amount ++ ")"
+  | cact_call to amount msg => "(call: " ++ show to ++ sep ++ show amount ++ sep ++
+      match @deserialize Msg _ msg with
+      | Some msg => str_of_msg msg
+      | None =>  "<FAILED DESERIALIZATION>"
+      end ++ ")"
+  end.
 
 Instance showSetup : Show Setup :=
 {|
@@ -96,3 +87,5 @@ Instance showState : Show Congress.State :=
             ++ "next_proposal_id: " ++ show (next_proposal_id s) ++ sep
             ++ "members: " ++ show (members s) ++ "}"
 |}.
+  
+End CongressPrinters.
