execution/tests/CongressTests/CongressTests.v
@@ -1,16 +1,14 @@
 From ConCert Require Import Blockchain LocalBlockchain Congress.
 From ConCert Require Import Serializable.
-From ConCert Require Import BoundedN ChainedList.
+From ConCert Require Import BoundedN ChainedList ResultMonad.
 Require Import Extras.
 
 From ConCert.Execution.QCTests Require Import
-  TestUtils ChainPrinters CongressGens CongressPrinters SerializablePrinters TraceGens.
+  TestUtils CongressGens TraceGens SerializablePrinters.
 
-Require Import ZArith Strings.Ascii Strings.String.
+Require Import ZArith.
 
 From QuickChick Require Import QuickChick. Import QcNotation.
-From ExtLib.Structures Require Import Functor Applicative.
-From ExtLib.Structures Require Import Monads.
 Import MonadNotation. Open Scope monad_scope.
 From Coq Require Import List. Import ListNotations.
 From Coq Require Import Strings.BinaryString.
@@ -19,20 +17,12 @@ From Coq Require Import Program.Basics.
 Require Import Containers.
 
 Notation "f 'o' g" := (compose f g) (at level 50).
-
 Definition LocalChainBase : ChainBase := TestUtils.LocalChainBase.
 
-
-(* chains for deploying congress with some existing members *)
 Definition chain1 : ChainBuilder := builder_initial.
-
-(* Creator created an empty block (and gets some coins) *)
-Definition chain2 : ChainBuilder :=
-  unpack_result (add_block chain1 []).
-
-(* Creator transfers 10 coins to person_1 *)
-Definition chain3 : ChainBuilder :=
-  unpack_result (add_block chain2 [build_act creator (act_transfer person_1 10)]).
+Definition chain2 : ChainBuilder := unpack_result (add_block chain1 []).
+Definition chain3 : ChainBuilder := unpack_result
+  (add_block chain2 [build_act creator (act_transfer person_1 10)]).
 
 Definition setup_rules :=
   {| min_vote_count_permille := 200; (* 20% of congress needs to vote *)
@@ -72,35 +62,21 @@ Definition create_proposal_call :=
 Definition chain6 : ChainBuilder :=
   unpack_result (add_block chain5 [build_act person_1 create_proposal_call]).
 
+Definition congress_chain := chain5.
+Definition congress_caddr := BoundedN.of_Z_const AddrSize 128%Z.
 
-Definition chain_with_congress_deployed : LocalChain := lcb_lc chain6. (* chain6 is from LocalBlockchainTests.v *)
-Definition congress_chain := chain_with_congress_deployed.
-Definition congress_contract_base_addr := BoundedN.of_Z_const AddrSize 128%Z.
+Definition gCongressChain max_acts_per_block congress_cb max_length := 
+  let act_depth := 2 in 
+  gChain congress_cb
+    (fun env act_depth => gCongressActionNew env act_depth congress_caddr) max_length act_depth max_acts_per_block.
 
-Extract Constant defNumDiscards => "(4 * defNumTests)".
+Definition forAllCongressChainTraces n :=
+  forAllChainState n congress_chain (gCongressChain 1).
 
-Definition gCongressChainTraceList max_acts_per_block lc length :=
-  gLocalChainTraceList_fix lc (fun lc _ =>
-    gCongressActionNew lc 2) length max_acts_per_block.
+Definition pre_post_assertion_congress P c Q :=
+  pre_post_assertion 5 congress_chain (gCongressChain 2) Congress.contract c P Q.
 
-Definition forAllCongressTraces n :=
-  forAllTraces n congress_chain (gCongressChainTraceList 1).
-Notation "{{ P }} c {{ Q }}" :=
-  (pre_post_assertion 10 congress_chain (gCongressChainTraceList 1) c P Q)( at level 50).
-
-Open Scope string_scope.
-Definition debug_congress {A : Type}
-                         `{Checkable A}
-                          (lc : LocalChain)
-                          (acts_opt : option (list Action))
-                          : A -> Checker :=
-  whenFail (
-    "LocalChain: " ++ show lc ++ nl ++
-    "members: " ++ show (congressContractsMembers lc) ++ nl ++
-    "active proposals: " ++ show (lc_proposals lc) ++ nl ++
-    "contract owners: " ++ show (lc_contract_owners lc)
-  ).
-Close Scope string_scope.
+Notation "{{ P }} c {{ Q }}" := (pre_post_assertion_congress P c Q) ( at level 50).
 
 Definition nr_cacts (msg : option Congress.Msg) :=
   match msg with
@@ -108,20 +84,12 @@ Definition nr_cacts (msg : option Congress.Msg) :=
   | _ => 0
   end.
 
-(* What this says is that the number of actions to be performed by the congress never increases
+(* This property states that the number of actions to be performed by the congress never increases
    more than the actions that are added in proposals, ie. actions can't appear out of nowhere. *)
 (* If we replace '<=' with '<' QC finds a counterexample - a proposal can contain an empty list of actions, so they are equal before/after add_proposal *)
 Definition receive_state_well_behaved state msg new_state (resp_acts : list ActionBody) :=
   num_cacts_in_state new_state + length resp_acts <=
   num_cacts_in_state state + nr_cacts msg.
-
-Lemma a : forall state msg new_state resp_acts,
-Dec (receive_state_well_behaved state msg new_state resp_acts).
-Proof.
-  intros. unfold receive_state_well_behaved.
-  constructor.
-  apply le_dec.
-Qed.
 
 Instance receive_state_well_behaved_dec_ {state : Congress.State}
                                         {msg : option Congress.Msg}
@@ -129,39 +97,35 @@ Instance receive_state_well_behaved_dec_ {state : Congress.State}
                                         {resp_acts : list ActionBody}
                                         : Dec (receive_state_well_behaved state msg new_state resp_acts).
 Proof.
-  intros.
-  unfold receive_state_well_behaved.
-  constructor.
+  intros;
+  unfold receive_state_well_behaved;
+  constructor;
   apply le_dec.
 Qed.
 
-(* Instance receive_state_well_behaved_checkable {state : Congress.State}
+Instance receive_state_well_behaved_checkable {state : Congress.State}
                                               {msg : option Congress.Msg}
                                               {new_state : Congress.State}
                                               {resp_acts : list ActionBody}
-                                              : Checkable (receive_state_well_behaved_inner state msg new_state resp_acts).
-Proof. apply testDec. Qed. *)
-
-
+                                              : Checkable (receive_state_well_behaved state msg new_state resp_acts).
+Proof. apply testDec. Qed.
 
 Definition receive_state_well_behaved_P (cctx : ContractCallContext)
                                         (old_state : Congress.State)
                                         (msg : Congress.Msg)
                                         (result : option (Congress.State * list ActionBody)) :=
-  match result with
+  checker match result with
   | Some (new_state, resp_acts) =>
     (receive_state_well_behaved old_state (Some msg) new_state resp_acts)?
-    (* checker (num_cacts_safe_P msg resp_acts old_state new_state)  *)
   | _ => false
   end.
 
 (* QuickChick (
   {{fun _ _ => true}}
-  Congress.contract
+  congress_caddr
   {{receive_state_well_behaved_P}}
 ). *)
 
-(* in 39 seconds: *)
 (* coqtop-stdout:+++ Passed 10000 tests (0 discards) *)
 
 
@@ -171,113 +135,53 @@ Definition state_proposals_proposed_in_valid_P (block_slot : nat) (state : Congr
   let proposals := map snd (FMap.elements (proposals state)) in
   forallb (fun p => proposed_in p <=? block_slot) proposals.
 
-Definition state_proposals_proposed_in_valid lc :=
-  let congress_state_map := lc_contract_state_deserialized Congress.State lc in
-  checker match FMap.find congress_contract_base_addr congress_state_map with
-  | Some congress_state =>
-    state_proposals_proposed_in_valid_P lc.(lc_slot) congress_state
-  | None => false
+Definition state_proposals_proposed_in_valid (cs : ChainState) :=
+  let state_opt := get_contract_state Congress.State cs congress_caddr in
+  whenFail (show cs.(env_chain))
+  match state_opt with
+  | Some state => checker (state_proposals_proposed_in_valid_P cs.(current_slot) state)
+  | None => checker true
   end.
-
-(* QuickChick (forAllCongressTraces 10 state_proposals_proposed_in_valid). *)
-
-(* in 37 seconds *)
+  
+(* QuickChick (forAllCongressChainTraces 5 state_proposals_proposed_in_valid). *)
 (* coqtop-stdout:+++ Passed 10000 tests (0 discards) *)
 
-
-(* sanity check *)
-Definition add_block_actions_succeeds_P c_opt actions_opt :=
-  isSomeCheck c_opt
-  (fun c =>
-    (debug_congress c actions_opt)
-      (match actions_opt with
-      | Some actions => (0 <? length actions) && isSome (my_add_block c actions)
-      | None => false
-      end)
-  ).
-
-Instance shrinkAction : Shrink Action := {| shrink a := [a] |}.
-
-(* another sanity check *)
-Definition check_add_two_blocks_succeeds :=
-  (forAll3
-    (optToVector 1 (gCongressActionNew chain_with_congress_deployed 2))
-    (fun actions => returnGen (my_add_block chain_with_congress_deployed actions))
-    (fun _ c_opt =>
-      bindGenOpt (returnGen c_opt)
-      (fun c =>
-        acts <- (optToVector 1 (gCongressActionNew c 2)) ;;
-        returnGen (Some acts)))
-    (fun _ c_opt actions_opt => add_block_actions_succeeds_P c_opt actions_opt)
-  ).
-
-(* QuickChick check_add_two_blocks_succeeds. *)
-(* coqtop-stdout:+++ Passed 10000 tests (0 discards) *)
-
-
-Definition reachableFrom_congress (lc : LocalChain) pf : Checker :=
-  @reachableFrom AddrSize lc (fun lc _ => gCongressChainTraceList 1 lc 2) pf.
+Definition reachableFrom_chaintrace_congress (cb : ChainBuilder) pf : Checker :=
+  reachableFrom_chaintrace cb (gCongressChain 1) pf.
 
 Notation "lc '~~>' pf" :=
-  (reachableFrom_congress lc pf)
+  (reachableFrom_chaintrace_congress lc pf)
   (at level 88, left associativity).
 
-Definition congress_has_votes_on_some_proposal lc :=
-  let congress_state_map := lc_contract_state_deserialized Congress.State lc in
-  match FMap.find congress_contract_base_addr congress_state_map with
+Definition congress_has_votes_on_some_proposal (cs : ChainState) :=
+  let state_opt := get_contract_state Congress.State cs congress_caddr in
+  match state_opt with
   | Some state =>
-    let proposals := map snd (FMap.elements (proposals state)) in
+       let proposals := map snd (FMap.elements (proposals state)) in
     existsb (fun proposal =>
       0 <? FMap.size proposal.(votes)
-    ) proposals
+    ) proposals 
   | None => false
   end.
 
-(* QuickChick (congress_chain ~~> congress_has_votes_on_some_proposal o next_lc_of_lcstep). *)
-(* coqtop-stdout:
-Begin Trace:
-step_action{
-  Action{
-    act_from: 12%256,
-    act_body: (act_call 128%256, 0, vote_against_proposal 1)}};;
-step_action{
-  Action{
-    act_from: 11%256,
-    act_body: (act_call 128%256, 5, create_proposal (call: 128%256, 4, create_proposal (call: 128%256, 4, vote_against_proposal 1)))}}
-End Trace
-Success - found witness satisfying the predicate!
-+++ Failed (as expected) after 15 tests and 0 shrinks. (0 discards)
-*)
+(* QuickChick (chain5 ~~> congress_has_votes_on_some_proposal). *)
+(* Success - found witness satisfying the predicate!
++++ Failed (as expected) after 7 tests and 0 shrinks. (0 discards) *)
 
 (* This assumes that in a previous block, there was an active proposal *)
-Definition congress_finished_a_vote (lc_step : @LocalChainStep AddrSize) :=
-  match lc_step with
-  | step_add_block _ _ _ => false
-  | step_action _ _ _ acts =>
-    let act_is_finish_vote (act : Action) := match act.(act_body) with
-                                             | act_call _ _ msg => match deserialize Congress.Msg _ msg with
-                                                                   | Some (Congress.finish_proposal _) => true
-                                                                   | _ => false end
-                                             | _ => false end in
-    existsb act_is_finish_vote acts
-  end.
+Definition congress_finished_a_vote (cs : ChainState) :=
+  let acts := cs.(chain_state_queue) in
+  let act_is_finish_vote (act : Action) := match act.(act_body) with
+                                           | act_call _ _ msg => 
+                                             match deserialize Congress.Msg _ msg with
+                                             | Some (Congress.finish_proposal _) => true
+                                             | _ => false
+                                             end
+                                           | _ => false 
+                                           end in
+    existsb act_is_finish_vote acts.
 
-(* QuickChick (congress_chain ~~> congress_finished_a_vote). *)
-(* Begin Trace:
-step_action{
-  Action{
-    act_from: 11%256,
-    act_body: (act_call 128%256, 3, finish_proposal 1)}};;
-step_action{
-  Action{
-    act_from: 12%256,
-    act_body: (
-      act_call 128%256, 0, create_proposal (
-        call: 128%256, 0, create_proposal (
-          call: 128%256, 2, change_rules Rules{
-            min_vote_count_permille: 450,
-            margin_needed_permille: 467,
-            debating_period_in_blocks: 2})))}}
-End Trace
-Success - found witness satisfying the predicate!
-+++ Failed (as expected) after 3 tests and 0 shrinks. (0 discards) *)
+
+(* QuickChick (chain5 ~~> congress_finished_a_vote). *)
+(* Success - found witness satisfying the predicate!
++++ Failed (as expected) after 14 tests and 0 shrinks. (0 discards) *)
