execution/tests/CongressTests/Congress_BuggyPrinters.v
@@ -7,15 +7,14 @@ Require Import ZArith Strings.Ascii Strings.String.
 
 From QuickChick Require Import QuickChick. Import QcNotation.
 From ExtLib.Structures Require Import Functor Applicative.
-From ExtLib.Structures Require Import Monads.
-Import MonadNotation. Open Scope monad_scope.
+(* From ExtLib.Structures Require Import Monads. *)
+(* Import MonadNotation. Open Scope monad_scope. *)
 From Coq Require Import List. Import ListNotations.
 From Coq Require Import Strings.BinaryString.
 From Coq Require Import Morphisms.
 From Coq Require Import Program.Basics.
 Require Import Containers.
 Notation "f 'o' g" := (compose f g) (at level 50).
-Definition LocalChainBase : ChainBase := TestUtils.LocalChainBase.
 Open Scope string_scope.
 
 Instance showRules : Show Rules :=
